examples/cellio/MainIAproof.v
@@ -1,5 +1,5 @@
 Require Import CRIS.
-Require Import CellioHeader CellioA MainHeader MainA MainI FooA InputA.
+Require Import CellioHeader CellioA MainHeader MainA MainI LibA LibA.
 
 Set Implicit Arguments.
 
@@ -11,8 +11,9 @@ Module MainIA. Section MainIA.
     λ _ st_src st_tgt, emp%I.
 
   Context (spc_s: string -> option fspec).
-  Context (FooInSpc: spc_incl FooAS.spc spc_s).
-  Context (InputInSpc: spc_incl InputAS.spc spc_s).
+  Context (LibInSpc: spc_incl LibAS.spc spc_s).
+  (* Context (FooInSpc: spc_incl FooAS.spc spc_s). *)
+  (* Context (InputInSpc: spc_incl InputAS.spc spc_s). *)
 
   Local Definition CellioA := (CellioA.t spc_s).
   Local Definition MainA := (MainA.t spc_s).
